src/later.v
@@ -1,0 +1,48 @@
+From iris.base_logic.lib Require Import iprop.
+From iris.base_logic Require Import bi.
+From iris.proofmode Require Import proofmode.
+From iris.itree Require Import wpi trace handler.
+From iris.base_logic.lib Require Export fancy_updates.
+From iris.proofmode Require Import proofmode.
+From ITree Require Import ITree.
+
+Variant laterE : Type → Type :=
+  | ELater : laterE ().
+
+Global Instance AnswerEqDecision_laterE :
+  AnswerEqDecision laterE.
+Proof. intros A [] [] []. by left. Qed.
+
+Section handler.
+  Context {Σ : gFunctors}.
+
+  Program Definition laterH : iHandler Σ laterE :=
+    IHandler (λ A e,
+      match e with
+      | ELater => λ Φ _, ▷ Φ ()
+      end
+    )%I _.
+  Next Obligation.
+    iIntros (??????) "HΦwand _". destruct e.
+    iIntros "HΦ". iNext. by iApply "HΦwand".
+  Qed.
+  Global Instance laterH_Sequential :
+    Sequential laterH.
+  Proof.
+    by iIntros (A [] Φ s) "HH".
+  Qed.
+End handler.
+
+Section wpi_later.
+  Context `{!invGS_gen hlc Σ} {E : Type → Type} {H : iHandler Σ E}.
+  Context `{laterE -< E} `{inH Σ laterE E laterH H}.
+
+  Lemma wpi_later M (Φ : () → iProp Σ) :
+    (▷ |={M}=> Φ ()) -∗
+    WPi (trigger ELater) @ H; M {{ Φ }}.
+  Proof.
+    iIntros "HΦ". iApply wpi_vis.
+    iApply fupd_mask_intro; first apply empty_subseteq. iIntros "Hfupd".
+    iApply is_inH. simpl. iNext. iApply wpi_ret. by iMod "Hfupd".
+  Qed.
+End wpi_later.
